adjust merge to use Racket-generated constants

rkt/merge.rkt
@@ -1,0 +1,26 @@
+#lang at-exp s-exp "tmonad.rkt"
+
+(Fixpoint
+ merge #:implicit @A{Set}
+ #:implicit @A_cmp{A -> A -> Prop}
+ @A_cmp_trans{Transitive A_cmp} @A_cmp_total{Total A_cmp} @A_cmp_dec{DecCmp A_cmp}
+ @xs{list A} @ys{list A}
+ #:measure "(length (xs ++ ys))"
+ #:returns @{list A}
+ (match (xs)
+   [(nil) => (<== ys)]
+   [(cons x xs′)
+    =>
+    (match (ys)
+      [(nil) => (<== xs)]
+      [(cons y ys′)
+       =>
+       (match ((A_cmp_dec x y))
+         [(left _) 
+          => 
+          (bind ((res (merge A_cmp_trans A_cmp_total A_cmp_dec xs′ ys)))
+                (<== (cons x res)))]
+         [(right _) 
+          => 
+          (bind ((res (merge A_cmp_trans A_cmp_total A_cmp_dec xs ys′)))
+                (<== (cons y res)))])])]))
