Makefile
@@ -69,7 +69,8 @@ tmonad-gen: insert/insert_log_gen.v \
             clrs/insert_gen.v \
             clrs/isort_gen.v \
             clrs/clength_gen.v \
-            clrs/split2_gen.v
+            clrs/split2_gen.v \
+            clrs/merge_gen.v
 
 insert/insert_log_gen.v: rkt/insert.rkt $(GEN_DEPS)
 	racket rkt/insert.rkt > insert/insert_log_gen.v
@@ -134,6 +135,8 @@ clrs/clength_gen.v: rkt/clength.rkt $(GEN_DEPS)
 	racket rkt/clength.rkt > clrs/clength_gen.v
 clrs/split2_gen.v: rkt/split2.rkt $(GEN_DEPS)
 	racket rkt/split2.rkt > clrs/split2_gen.v
+clrs/merge_gen.v: rkt/merge.rkt $(GEN_DEPS)
+	racket rkt/merge.rkt > clrs/merge_gen.v
 
 Makefile.coq: tmonad-gen Makefile $(VS)
 	coq_makefile -R . Braun $(VS) -o Makefile.coq
